coq/theories/imp2asm/ImpToASMCodegen.v
@@ -341,8 +341,6 @@ Function c_cmd (c : cmd) (l : nat) (fs : f_lookup) (vs : v_stack) : (asm_appl * 
     let/d jump_to_c2 := List [ASMSyntax.Jump Always l2] in
     let/d jump_to_end := List [ASMSyntax.Jump Always l3] in
     let/d asmres := jump_to_start +++ jump_to_c1 +++ jump_to_c2 +++ asm1 +++ asm2 +++ jump_to_end +++ asm3 in
-    (* TODO(kπ): Cannot know the result `vs` statically. Is there a better way to compile `if`s? *)
-    (*           Should we manually drop the additional stuff from the stack *)
     (asmres, l3)
   | While tst body =>
     let/d '(asm1, l1) := c_test_jump tst (l + 1) (l + 2) (l + 3) vs in
@@ -352,7 +350,6 @@ Function c_cmd (c : cmd) (l : nat) (fs : f_lookup) (vs : v_stack) : (asm_appl * 
     let/d jump_to_body := List [ASMSyntax.Jump Always l1] in
     let/d jump_to_end := List [ASMSyntax.Jump Always (l2 + 1)] in
     let/d asmres := jump_to_tst +++ jump_to_body +++ jump_to_end +++ asm1 +++ asm2 +++ jump_to_beginning in
-    (* TODO(kπ): Same as with if: what's the correct result `vs` here? *)
     (asmres, l2+1)
   | Call n f es =>
     let/d target := lookup f fs in
